examples/graph/theories/SPProofs.v
@@ -1,0 +1,427 @@
+Require Import Data.Graph.Inductive.Query.SP.
+Require Import Lex.
+Require Import Path.
+Require Import Data.Graph.Inductive.Internal.Heap.
+Require Import Omega.
+Require Import Equations.Equations.
+Require Import Coq.Bool.Bool.
+Require Import Data.Graph.Inductive.Graph.
+Require Import Coq.Lists.List.
+Require Import DeferredFix.
+Require Import GHC.Num.
+Import GHC.Num.Notations.
+Require Import HeapProofs.
+
+
+(* Inductive relation*)
+Section Ind.
+
+Context {a : Type} {b : Type} { gr : Type -> Type -> Type} {Hgraph : Graph.Graph gr} {Hlaw : Graph.LawfulGraph gr}
+{Hnum: GHC.Num.Num b} {Heq: Base.Eq_ b} {HOrd: Base.Ord b} {Hreal: @GHC.Real.Real b Hnum Heq HOrd}
+{Heq': Base.Eq_ a} {HOrd': Base.Ord a} {Herr: Err.Default (b)}.
+
+Program Instance path_default : Err.Default (Graph.LPath b).
+Next Obligation.
+constructor. apply nil.
+Defined.
+
+(*Well formed lexicographic measure*)
+Definition natNodes := (@Path.natNodes a b gr Hgraph).
+
+Definition natNodes_lt (x y : gr a b) := natNodes x < natNodes y.
+
+Definition natNodes_eq (x y : gr a b) := natNodes x = natNodes y.
+(*Definition list_length_lt {a b} (x y : list a) := size x < size y*)
+Definition heap_length_lt (x y : Heap b (Graph.LPath b)) := (Heap.size x) < (Heap.size y).
+ (*list_lsize (toList x) (toList y).*)
+
+Definition bf_measure_heap:=
+  lex _ _ (natNodes_lt) natNodes_eq (heap_length_lt).
+
+Lemma well_founded_bf_measure_heap : well_founded (bf_measure_heap).
+Proof.
+  intros. eapply WF_lex.
+  - apply f_nat_lt_wf.
+  - apply f_nat_lt_wf.
+  - unfold RelationClasses.Transitive. intros. unfold natNodes_eq in *; omega.
+  - intros. unfold natNodes_eq in *. unfold natNodes_lt in *. destruct H. destruct H.
+    omega.
+  - unfold RelationClasses.Symmetric. intros. unfold natNodes_eq in *. omega.
+Qed. 
+
+Instance need_this_for_equations : WellFounded (bf_measure_heap).
+Proof.
+  unfold WellFounded. apply well_founded_bf_measure_heap.
+Defined.
+
+
+(*TODO: Dont copy this*)
+Lemma match_none_size: forall g v g',
+  match_ v g = (None, g') -> natNodes g = natNodes g'.
+Proof.
+  intros. pose proof (match_remain_none g). erewrite H0. reflexivity. apply H.
+Qed.  
+
+Definition state : Type := (gr a b) * (Heap b (LPath b)) * (list (LPath b)).
+
+Definition get_graph (s: state) :=
+  match s with
+  | (g, _, _) => g
+  end.
+
+Definition get_heap (s: state) :=
+  match s with
+  | (_, h, _) => h
+end.
+
+Definition get_paths (s: state) :=
+  match s with
+  | (_, _, p) => p
+  end.
+
+
+(*How to step from 1 state to another. The inductive definiction makes it easier to use as
+  an assumption in proofs*)
+Inductive sp_step : state -> state -> Prop :=
+  | sp_find: forall (g: gr a b) (v : Node) (c: Context a b) (g': gr a b) (a' : b) 
+      (d: b) (t: list (Node * b)) (h' h : Heap b (LPath b)) (p : list (LPath b)) (p' : (LPath b)),
+      isEmpty g = false ->
+      match_ v g = (Some c, g') ->
+      splitMinT h = Some ((a', p'), h') ->
+      p' = LP ((v,d) :: t) ->
+      sp_step (g, h, p) (g', mergeAll (h' :: expand d p' c), p ++ p' :: nil)
+  | sp_skip : forall (g: gr a b) (v: Node) (g': gr a b) (h h' : Heap b (LPath b))
+     (p: list (LPath b)) (p': (LPath b)) (a' : b),
+      isEmpty g = false ->
+      match_ v g = (None, g') ->
+      splitMinT h = Some ((a', p'), h') ->
+      sp_step (g, h, p) (g', h', p).
+
+Definition start (g : gr a b) (v: Graph.Node) : state := (g, Heap.unit #0 (LP ((v, #0) :: nil)), nil).
+
+(*A valid state is any state that can be reached from the start state.*)
+Inductive valid : state -> (gr a b) -> Node -> Prop :=
+  | v_start : forall g v, vIn g v = true -> valid (start g v) g v
+  | v_step : forall s s' v g, valid s' g v -> sp_step s' s -> valid s g v.
+
+(*From Software Foundations*)
+Definition relation (X : Type) := X -> X -> Prop.
+
+Inductive multi {X : Type} (R : relation X) : relation X :=
+  | multi_refl : forall (x : X), multi R x x
+  | multi_step : forall (x y z : X),
+                    R x y ->
+                    multi R y z ->
+                    multi R x z.
+
+Theorem multi_R : forall (X : Type) (R : relation X) (x y : X),
+    R x y -> (multi R) x y.
+Proof.
+  intros X R x y H.
+  apply multi_step with y. apply H. apply multi_refl.
+Qed.
+
+Theorem multi_trans :
+  forall (X : Type) (R : relation X) (x y z : X),
+      multi R x y ->
+      multi R y z ->
+      multi R x z.
+Proof.
+  intros X R x y z G H.
+  induction G.
+    - (* multi_refl *) assumption.
+    - (* multi_step *)
+      apply multi_step with y. assumption.
+      apply IHG. assumption.
+Qed.
+
+Definition sp_multi (s1 s2 : state):= multi (sp_step) s1 s2.
+
+Lemma multi_valid: forall s1 s2 g v,
+  valid s1 g v ->
+  sp_multi s1 s2 ->
+  valid s2 g v.
+Proof.
+  intros. induction H0. assumption. apply IHmulti. eapply v_step. apply H. assumption.
+Qed.
+
+Definition done (s: state) := Heap.isEmpty (get_heap s) || isEmpty (get_graph s).
+
+(*The executable, tail recursive version of this, which we will prove equivalent to the hs-to-coq version*)
+Section Exec.
+
+Program Instance default_state : Default state.
+Next Obligation.
+unfold state. apply ((empty, Heap.Empty, nil)).
+Defined.
+
+
+Equations sp_tail (s: state) : state by wf (get_heap s, get_graph s) (bf_measure_heap) :=
+  sp_tail (g, h, l) =>  if bool_dec ((Heap.isEmpty h) || (@Graph.isEmpty gr Hgraph a b g)) true then (g, h, l) else
+                        match (splitMinT h) as s return ((splitMinT h = s) -> _) with
+                          |Some ((_, p), h') => fun H : (splitMinT h = Some ((_, p), h')) =>
+                          match p as p'' return ((p = p'') -> _) with
+                            | LP nil => fun H : (p = LP nil) => Err.patternFailure
+                            | LP ((v,d) :: t) => fun H : (p = LP ( (v,d) :: t)) =>
+                                match (match_ v g) as y return ((match_ v g = y) -> _ ) with
+                                | (Some c, g') => fun H : (match_ v g) = (Some c, g') => sp_tail (g', mergeAll (h' :: expand d p c), l ++ (p :: nil))
+                                | (None, g') => fun H: (match_ v g) = (None, g') => sp_tail (g', h', l)
+                                 end (eq_refl)
+                            end (eq_refl)
+                           | None => fun H : (splitMinT h = None) => Err.patternFailure
+                         end (eq_refl).
+Next Obligation.
+simpl. destruct c. destruct p. destruct p. unfold Base.map. apply lex1. unfold natNodes_lt. eapply match_decr_size.
+symmetry. apply H.
+Defined.
+Next Obligation.
+apply lex2. symmetry. unfold natNodes_eq. eapply match_none_size. apply H. unfold heap_length_lt.
+unfold splitMin in H0. destruct h. simpl in n. contradiction. inversion H0; subst.
+rewrite (mergeAll_size l5). simpl. omega.
+Defined.
+
+Definition expand_sp_tail :=
+fun s : gr a b * Heap b (LPath b) * list (LPath b) =>
+let (p, l) := s in
+(let (g, h) := p in
+ fun l0 : list (LPath b) =>
+ if bool_dec (Heap.isEmpty h || isEmpty g) true
+ then (g, h, l0)
+ else
+  match splitMinT h as s0 return (splitMinT h = s0 -> gr a b * Heap b (LPath b) * list (LPath b)) with
+  | Some p0 =>
+      let (p1, h') as p1 return (splitMinT h = Some p1 -> gr a b * Heap b (LPath b) * list (LPath b)) := p0 in
+      let (b0, p2) as p2 return (splitMinT h = Some (p2, h') -> gr a b * Heap b (LPath b) * list (LPath b)) :=
+        p1 in
+      fun _ : splitMinT h = Some (b0, p2, h') =>
+      match p2 as p'' return (p2 = p'' -> gr a b * Heap b (LPath b) * list (LPath b)) with
+      | LP unLPath =>
+          match unLPath as unLPath0 return (p2 = LP unLPath0 -> gr a b * Heap b (LPath b) * list (LPath b)) with
+          | nil => fun _ : p2 = LP nil => patternFailure
+          | l1 :: t =>
+              let (v, d) as l2 return (p2 = LP (l2 :: t) -> gr a b * Heap b (LPath b) * list (LPath b)) := l1 in
+              fun _ : p2 = LP ((v, d) :: t) =>
+              (let (m, g') as y return (match_ v g = y -> gr a b * Heap b (LPath b) * list (LPath b)) :=
+                 match_ v g in
+               match m as m0 return (match_ v g = (m0, g') -> gr a b * Heap b (LPath b) * list (LPath b)) with
+               | Some c =>
+                   fun _ : match_ v g = (Some c, g') =>
+                   sp_tail (g', mergeAll (h' :: expand d p2 c), l0 ++ p2 :: nil)
+               | None => fun _ : match_ v g = (None, g') => sp_tail (g', h', l0)
+               end) eq_refl
+          end
+      end eq_refl
+  | None => fun _ : splitMinT h = None => patternFailure
+  end eq_refl) l.
+
+Lemma unfold_sp_tail: forall s,
+  sp_tail s = expand_sp_tail s.
+Proof.
+  intros. unfold expand_sp_tail. apply sp_tail_elim; intros; reflexivity.
+Qed.
+
+(*This is equivalent to repeatedly stepping with the sp_step inductive relation. We prove this by proving that
+  bfs_tail represents a multistep to a done state. So when we start with the start state, we get a valid
+  done state. We will later prove that all valid done states are equivalent, so we can prove claims about bfs_tail
+  by considering valid done states in general*)
+
+Lemma heap_not_none: forall s v g k,
+  valid s v g ->
+  ~ In_Heap (k, (LP nil)) (get_heap s).
+Proof.
+  intros. induction H; intro.
+  - simpl in H0. destruct H0. inversion H0. destruct H0.
+  - inversion H0; subst.
+    + unfold get_heap in H1. rewrite in_heap_mergeAll in H1. unfold fold_right in H1.
+      destruct H1. simpl in IHvalid. apply IHvalid. pose proof (in_heap_splitMin (k, (LP nil)) h h' a' (LP ((v0, d) :: t))).
+      rewrite H5. right. assumption. intro. subst. simpl in H4. inversion H4. 
+      rewrite <- splitMin_equiv in H4. inversion H4. reflexivity. intro. subst. simpl in H4. inversion H4.
+      assert (fold_right (fun x acc => In_Heap (k, LP nil) x \/ acc) False (expand d (LP ((v0, d) :: t)) c)).
+      unfold fold_right. apply H1. clear H1. rewrite in_heap_exists in H5.
+      destruct H5. destruct H1. simpl in IHvalid.
+      simpl in H1. destruct c. destruct p0. destruct p0. unfold Base.map in H1.
+      rewrite in_map_iff in H1. destruct H1. destruct x0. destruct H1.
+      rewrite <- H1 in H5. unfold unit in H5. simpl in H5. destruct H5. inversion H5. destruct H5.
+    + simpl in IHvalid. simpl in H1. destruct h. simpl in H4. inversion H4. simpl in H4. 
+      inversion H4. subst. simpl in IHvalid. rewrite in_heap_mergeAll in H1. apply IHvalid.
+      right. rewrite <- in_heap_equiv. apply H1. 
+Qed.
+
+Lemma sp_tail_multi: forall s v g,
+  valid s v g ->
+  sp_multi s (sp_tail s).
+Proof.
+  intros. destruct s as[r p].
+  remember (snd r, fst r) as r'. generalize dependent r. revert p. 
+  induction r' using (well_founded_induction (well_founded_bf_measure_heap)).
+  intros. destruct r' as [q h]. inversion Heqr'; subst. clear Heqr'. destruct r as [g' h].
+  rewrite unfold_sp_tail. unfold expand_sp_tail. destruct (Heap.isEmpty h) eqn : E. apply multi_refl.
+  destruct (isEmpty g') eqn : GE. simpl. apply multi_refl. destruct (bool_dec (false || false) true) eqn : U.
+  simpl in e. inversion e. destruct (splitMinT h) eqn : S. destruct p0. destruct p0. 
+  destruct l. destruct h. inversion S. simpl in S. inversion S. subst. destruct unLPath.
+  exfalso. eapply heap_not_none. apply H0. simpl.  left. reflexivity. destruct l. 
+  destruct (match_ n0 g') eqn : M. destruct m.
+  - eapply multi_step. eapply sp_find. assumption. apply M. simpl. reflexivity.
+    reflexivity. eapply H. apply lex1. 3 :{ reflexivity. } unfold natNodes_lt. simpl.
+    eapply match_decr_size. symmetry. apply M. eapply v_step. apply H0. eapply sp_find.
+    apply GE. apply M. simpl. reflexivity. reflexivity.
+  - eapply multi_step. eapply sp_skip. apply GE. apply M. simpl. reflexivity.
+    eapply H. 3 : { reflexivity. }  apply lex2. simpl. symmetry. eapply match_none_size.
+    apply M. simpl. unfold heap_length_lt. rewrite mergeAll_size. simpl.
+    omega. eapply v_step. apply H0. eapply sp_skip. assumption. apply M. simpl. reflexivity.
+  - destruct h. simpl in E. inversion E. simpl in S. inversion S.
+Qed.
+
+Lemma sp_tail_done: forall s v g,
+  valid s v g ->
+  done (sp_tail s) = true.
+Proof.
+  intros. unfold done. destruct s as[r p].
+  remember (snd r, fst r) as r'. generalize dependent r. revert p. 
+  induction r' using (well_founded_induction (well_founded_bf_measure_heap)).
+  intros. destruct r. simpl in Heqr'. destruct r'. inversion Heqr'. subst. clear Heqr'.
+  rewrite unfold_sp_tail. unfold expand_sp_tail. destruct h. simpl. reflexivity.
+  destruct (isEmpty g0) eqn : E. simpl. assumption.
+  destruct (bool_dec (Heap.isEmpty (Heap.Node b0 l l0) || false) true) eqn : ?. simpl in Heqs. inversion Heqs.
+  clear Heqs. destruct (splitMinT (Heap.Node b0 l l0)) eqn : Min. simpl in Min. destruct p0. destruct p0.
+  inversion Min; subst. clear Min. destruct l1. destruct unLPath.
+  exfalso. eapply heap_not_none. apply H0. simpl. left. reflexivity. destruct l. 
+  destruct (match_ n0 g0) eqn : M. destruct m.
+  -  remember (sp_tail (g1, mergeAll (mergeAll l0 :: expand b0 (LP ((n0, b0) :: unLPath)) c),
+        p ++ LP ((n0, b0) :: unLPath) :: nil)) as s'. eapply H.  3 : { reflexivity. } apply lex1.
+    simpl. eapply match_decr_size. symmetry. apply M. eapply v_step. apply H0. eapply sp_find.
+    symmetry. symmetry; assumption. apply M. simpl. reflexivity. reflexivity.
+  - eapply H. 3 : { reflexivity. } apply lex2. simpl. symmetry. eapply match_none_size. apply M.
+    simpl. unfold heap_length_lt. rewrite mergeAll_size.  simpl. omega. eapply v_step. apply H0.
+    eapply sp_skip. assumption. apply M. simpl. reflexivity.
+  - simpl in Min. inversion Min.
+Qed.
+
+End Exec.
+
+(*Prove equivalence with equations version*)
+
+Equations dijkstra' (x: (Heap b (Graph.LPath b)) * (gr a b)) : list (Graph.LPath b) by wf x (bf_measure_heap) :=
+  dijkstra' (h, g) := if bool_dec ((Heap.isEmpty h) || (Graph.isEmpty g)) true then nil else
+                        match (splitMinT h) as s return ((splitMinT h = s) -> _) with
+                          |Some ((_, p), h') => fun H : (splitMinT h =  Some ((_, p), h')) =>
+                          match p as p' return ((p = p') -> _) with
+                            | LP nil => fun H : (p = LP nil) => Err.patternFailure
+                            | LP ((v,d) :: t) => fun H : (p = LP ( (v,d) :: t)) =>
+                                match (match_ v g) as y return ((match_ v g = y) -> _ ) with
+                                | (Some c, g') => fun H : (match_ v g) = (Some c, g') => p :: dijkstra' (mergeAll (h' :: expand d p c), g')
+                                | (None, g') => fun H: (match_ v g) = (None, g') => dijkstra' (h', g')
+                                 end (eq_refl)
+                            end (eq_refl)
+                          | None => fun H : (splitMinT h = None) => Err.patternFailure
+                         end (eq_refl).
+Next Obligation.
+simpl. destruct c. destruct p. destruct p. unfold Base.map. apply lex1. unfold natNodes_lt. eapply match_decr_size.
+symmetry. apply H.
+Defined.
+Next Obligation.
+apply lex2. symmetry. unfold natNodes_eq. eapply match_none_size. apply H. unfold heap_length_lt.
+unfold splitMin in H0. destruct h. simpl in n. contradiction. inversion H0; subst.
+rewrite (mergeAll_size l4). simpl. omega.
+Defined.
+
+
+Definition expand_dijkstra' := 
+fun x : Heap b (LPath b) * gr a b =>
+let (h, g) := x in
+if bool_dec (Heap.isEmpty h || isEmpty g) true
+then nil
+else
+ match splitMinT h as s return (splitMinT h = s -> list (LPath b)) with
+ | Some p0 =>
+     let (p1, h') as p1 return (splitMinT h = Some p1 -> list (LPath b)) := p0 in
+     let (b0, p) as p2 return (splitMinT h = Some (p2, h') -> list (LPath b)) := p1 in
+     fun _ : splitMinT h = Some (b0, p, h') =>
+     match p as p' return (p = p' -> list (LPath b)) with
+     | LP unLPath =>
+         match unLPath as unLPath0 return (p = LP unLPath0 -> list (LPath b)) with
+         | nil => fun _ : p = LP nil => patternFailure
+         | l :: t =>
+             let (v, d) as l0 return (p = LP (l0 :: t) -> list (LPath b)) := l in
+             fun _ : p = LP ((v, d) :: t) =>
+             (let (m, g') as y return (match_ v g = y -> list (LPath b)) := match_ v g in
+              match m as m0 return (match_ v g = (m0, g') -> list (LPath b)) with
+              | Some c => fun _ : match_ v g = (Some c, g') => p :: dijkstra' (mergeAll (h' :: expand d p c), g')
+              | None => fun _ : match_ v g = (None, g') => dijkstra' (h', g')
+              end) eq_refl
+         end
+     end eq_refl
+ | None => fun _ : splitMinT h = None => patternFailure
+ end eq_refl.
+
+Lemma unfold_dijkstra' : forall x,
+  expand_dijkstra' x = dijkstra' x.
+Proof.
+  intros. unfold expand_dijkstra'. apply dijkstra'_elim. reflexivity.
+Qed. 
+
+Lemma dijkstra'_equiv: forall h g,
+  dijkstra h g = dijkstra' (h, g).
+Proof.
+  intros. remember (h,g) as x. generalize dependent g. revert h.
+  induction x using (well_founded_induction (well_founded_bf_measure_heap)).
+  intros. destruct x. inversion Heqx. subst. clear Heqx. unfold dijkstra.
+  rewrite <- unfold_dijkstra'. simpl. unfold deferredFix2. unfold curry.
+  rewrite (deferredFix_eq_on _ (fun x => True) ( (bf_measure_heap) )).
+  - simpl. destruct (Heap.isEmpty h) eqn : E; simpl. reflexivity.
+    destruct (isEmpty g) eqn : G; simpl. reflexivity. destruct h. simpl in E. inversion E.
+    simpl. destruct l. destruct (unLPath). reflexivity. destruct l. 
+    destruct (match_ n g) eqn : M. destruct m.
+    +  unfold dijkstra in H. unfold deferredFix2 in H. unfold curry in H. erewrite H. reflexivity.
+        apply lex1. unfold natNodes_lt. eapply match_decr_size. symmetry. apply M. reflexivity.
+    + unfold dijkstra in H. unfold deferredFix2 in H. unfold curry in H. erewrite H. reflexivity.
+      apply lex2. unfold natNodes_eq. symmetry. eapply match_none_size. apply M. unfold heap_length_lt.
+      simpl. rewrite (mergeAll_size l0). omega. reflexivity.
+  - apply well_founded_bf_measure_heap.
+  - unfold recurses_on. intros. unfold uncurry. destruct x. destruct (Heap.isEmpty h1) eqn : H';
+     simpl. reflexivity. destruct (isEmpty g1) eqn : G'; simpl. reflexivity. destruct h1. simpl in H'.
+    inversion H'. simpl. destruct l; try(reflexivity). destruct unLPath; try(reflexivity). destruct l.
+    destruct (match_ n g1) eqn : M'. destruct m.
+    + erewrite H1. reflexivity. auto. apply lex1. unfold natNodes_lt. eapply match_decr_size.
+      symmetry. apply M'.
+    + apply H1. auto. apply lex2. unfold natNodes_eq. symmetry. eapply match_none_size. apply M'.
+      unfold heap_length_lt. rewrite (mergeAll_size l0). simpl. omega.
+  - auto.
+Qed.
+
+(*Equivalence with tail recursive version*)
+Lemma leveln_tail_equiv: forall g h l,
+  (forall k, ~In_Heap (k, LP nil) h) ->
+  get_paths (sp_tail (g, h, l)) = l ++ dijkstra' (h, g).
+Proof.
+  intros. remember (h, g) as x. generalize dependent h. revert g. revert l.
+  induction x using (well_founded_induction (well_founded_bf_measure_heap)).
+  intros. destruct x; inversion Heqx; subst; clear Heqx.
+  rewrite <- unfold_dijkstra'. rewrite unfold_sp_tail. simpl.
+  destruct h eqn : H'. 
+  - simpl. rewrite app_nil_r. reflexivity.
+  - simpl. destruct (isEmpty g) eqn : G. 
+    + simpl. rewrite app_nil_r. reflexivity.
+    + simpl. destruct l0. destruct unLPath. exfalso. eapply H0. simpl. left. reflexivity.
+      destruct l0. destruct (match_ n g) eqn : M. destruct m.
+      * erewrite H. rewrite <- app_assoc. reflexivity. apply lex1. unfold natNodes_lt. eapply match_decr_size.
+        symmetry. apply M. intros. intro. destruct (expand b1 (LP ((n, b1) :: unLPath)) c) eqn : E; rewrite E in H1.
+        -- rewrite in_heap_mergeAll in H1. eapply H0. simpl. right. rewrite <- in_heap_equiv. apply H1.
+        -- simpl in E. destruct c. destruct p. destruct p.
+           rewrite in_heap_merge in H1. destruct H1.
+           ++ rewrite in_heap_merge in H1. destruct H1.
+              ** rewrite in_heap_mergeAll in H1. eapply H0. simpl. right. rewrite <- in_heap_equiv. apply H1.
+              ** destruct a0. simpl in E. inversion E. simpl in E. inversion E. destruct p. 
+                 rewrite <- H3 in H1. simpl in H1. destruct H1. inversion H1. destruct H1.
+          ++ destruct a0. simpl in E. inversion E. simpl in E. inversion E. rewrite in_heap_mergeAll in H1.
+             rewrite in_heap_exists in H1. destruct H1. rewrite <- H4 in H1. destruct H1. 
+             unfold Base.map in H1. rewrite in_map_iff in H1. destruct H1. destruct x0.
+             destruct H1. rewrite <- H1 in H2. unfold unit in H2. simpl in H2. destruct H2. inversion H2.
+             destruct H2.
+        -- reflexivity.
+      * erewrite H. reflexivity. apply lex2. unfold natNodes_eq. symmetry. eapply match_none_size. apply M.
+        unfold heap_length_lt. rewrite mergeAll_size. simpl. omega. intros. intro.
+        apply (H0 k). right. rewrite in_heap_mergeAll in H1. rewrite in_heap_equiv in H1. apply H1. reflexivity.
+Qed.
+
+End Ind.
